ObcToClight/SepInvariant.v
@@ -14,7 +14,14 @@ Require Import ZArith.BinInt.
 
 Require Import Program.Tactics.
 
-Require Import Sep Syn Sem Tra.
+Require Import Rustre.Obc.Syntax.
+Require Import Rustre.Obc.Semantics.
+Require Import Rustre.ObcToClight.MoreSeparation.  
+Require Import Rustre.ObcToClight.Translation.
+Require Import Rustre.Ident.
+Require Import Rustre.ObcToClight.Interface.
+
+Module Export Sem := SemanticsFun Ids Op OpAux Syn.
 
 Open Scope list.
 Open Scope sep_scope.
@@ -45,37 +52,34 @@ Proof.
 Qed.
 
 Remark match_find_var_det:
-  forall me ve x v1 v2,
+  forall ve x v1 v2,
     match_value ve x v1 ->
-    find_var (me, ve) x v2 ->
+    PM.find x ve = Some v2 ->
     v1 = v2.
 Proof.
-  unfold match_value, find_var; simpl.
+  unfold match_value; simpl.
   intros ** Hm Hf.
-  destruct (PM.find x ve).
-  - subst; inv Hf; reflexivity.
-  - discriminate.
+  now rewrite Hf in Hm.
 Qed.
-
 
 Ltac app_match_find_var_det :=
   match goal with
-  | H1: find_var (?me, ?ve) ?x ?v1,
+  | H1: PM.find ?x ?ve = Some ?v1,
         H2: match_value ?ve ?x ?v2 |- _ =>
-    assert (v2 = v1) by (apply (match_find_var_det _ _ _ _ _ H2 H1)); subst v1; clear H2
+    assert (v2 = v1) by (apply (match_find_var_det _ _ _ _ H2 H1)); subst v1; clear H2
   end.
 
-Definition instance_match (me: menv) (i: ident): menv :=
+Definition instance_match (me: heap) (i: ident): heap :=
   match mfind_inst i me with
-  | None => m_empty
+  | None => hempty
   | Some i => i
   end.
 
 Lemma instance_match_empty:
-  forall x, instance_match m_empty x = m_empty.
+  forall x, instance_match hempty x = hempty.
 Proof.
   intros. unfold instance_match, mfind_inst; simpl.
-  rewrite PM.gempty. reflexivity.
+  now rewrite PM.gempty. 
 Qed.
 
 Remark field_offset_rec_in_range':
@@ -101,11 +105,13 @@ Proof.
   unfold field_offset; intros.
   eapply field_offset_rec_in_range'; eauto.
 Qed.
-  
+
+Definition chunk_of_type ty := AST.chunk_of_type (Ctypes.typ_of_type (cltype ty)).
+
 Section Staterep.
   Variable ge : composite_env.
 
-  Definition staterep_mems (cls: class) (me: menv) (b: block) (ofs: Z) (xty: ident * typ) :=
+  Definition staterep_mems (cls: class) (me: heap) (b: block) (ofs: Z) (xty: ident * type) :=
     let (x, ty) := xty in
     match field_offset ge x (make_members cls) with
     | Errors.OK d =>
@@ -114,7 +120,7 @@ Section Staterep.
     end.
 
   Fixpoint staterep
-           (p: program) (clsnm: ident) (me: menv) (b: block) (ofs: Z): massert :=
+           (p: program) (clsnm: ident) (me: heap) (b: block) (ofs: Z): massert :=
     match p with
     | nil => sepfalse
     | cls :: p' =>
@@ -132,7 +138,7 @@ Section Staterep.
       else staterep p' clsnm me b ofs
     end.
 
-  Definition staterep_objs (p': program) (cls: class) (me: menv) (b: block) (ofs: Z) (o: ident * ident) :=
+  Definition staterep_objs (p': program) (cls: class) (me: heap) (b: block) (ofs: Z) (o: ident * ident) :=
     let (i, c) := o in
     match field_offset ge i (make_members cls) with
     | Errors.OK d =>
@@ -246,9 +252,7 @@ Lemma co_members_alignof:
   forall env co,
     composite_consistent env co ->
     attr_alignas (co_attr co) = None ->
-    Forall (fun (x: ident * type) =>
-              (alignof env (snd x) | co_alignof co))
-           (co_members co).
+    Forall (fun x => (alignof env (snd x) | co_alignof co)) (co_members co).
 Proof.
   intros env co Henv Hattr.
   rewrite co_consistent_alignof with (1:=Henv).
@@ -296,8 +300,8 @@ Qed.
 
 Lemma sizeof_translate_chunk:
   forall gcenv t,
-    Ctypes.access_mode t = Ctypes.By_value (chunk_of_type t) ->
-    sizeof gcenv t = Memdata.size_chunk (chunk_of_type t).
+    Ctypes.access_mode (cltype t) = Ctypes.By_value (chunk_of_type t) ->
+    sizeof gcenv (cltype t) = Memdata.size_chunk (chunk_of_type t).
 Proof.
   destruct t;
   (destruct i, s || destruct f || idtac);
@@ -306,8 +310,8 @@ Qed.
 
 Lemma align_chunk_divides_alignof_type:
   forall gcenv t,
-    Ctypes.access_mode t = Ctypes.By_value (chunk_of_type t) ->
-    (Memdata.align_chunk (chunk_of_type t) | alignof gcenv t).
+    Ctypes.access_mode (cltype t) = Ctypes.By_value (chunk_of_type t) ->
+    (Memdata.align_chunk (chunk_of_type t) | alignof gcenv (cltype t)).
 Proof.
   destruct t;
   (destruct i, s || destruct f || idtac);
@@ -316,12 +320,12 @@ Proof.
 Admitted.
 
 Lemma in_translate_param_chunked:
-  forall ge (flds: list (ident * typ)) x ty,
-    Ctypes.access_mode ty = Ctypes.By_value (chunk_of_type ty) ->
-    In (x, ty) flds ->
+  forall ge (flds: list (ident * Ctypes.type)) x ty,
+    Ctypes.access_mode (cltype ty) = Ctypes.By_value (chunk_of_type ty) ->
+    In (x, cltype ty) flds ->
     exists chunk,
-      access_mode ty = By_value chunk
-      /\ (Memdata.align_chunk chunk | alignof ge ty).
+      access_mode (cltype ty) = By_value chunk
+      /\ (Memdata.align_chunk chunk | alignof ge (cltype ty)).
 Proof.
   intros ** ? Hin.
   exists (chunk_of_type ty).
@@ -358,11 +362,13 @@ Section StateRepProperties.
       NoDupMembers (make_members cls) ->
       forall x ty,
         In (x, ty) cls.(c_mems) ->
-        field_type x (make_members cls) = Errors.OK ty.
+        field_type x (make_members cls) = Errors.OK (cltype ty).
   Proof.
     intros ** Hfind Hndup ? ? Hin.
     apply in_field_type with (1:=Hndup).
-    unfold make_members. apply in_app_iff. now left.
+    unfold make_members, translate_param. apply in_app_iff.
+    left. rewrite in_map_iff.
+    exists (x, ty); split; auto.
   Qed.
 
   Lemma field_translate_obj_type:
@@ -386,13 +392,13 @@ Section StateRepProperties.
       WelldefClasses prog ->
       find_class clsnm prog <> None ->
       range b 0 (sizeof gcenv (type_of_inst clsnm)) -*>
-            staterep gcenv prog clsnm m_empty b 0.
+            staterep gcenv prog clsnm hempty b 0.
   Proof.
     intros ** Hwdef Hfind.
     cut (forall lo,
            (alignof gcenv (type_of_inst clsnm) | lo) ->
            massert_imp (range b lo (lo + sizeof gcenv (type_of_inst clsnm)))
-                       (staterep gcenv prog clsnm m_empty b lo)).
+                       (staterep gcenv prog clsnm hempty b lo)).
     - intro HH; apply HH; apply Z.divide_0_r.
     - clear TRANSL.
 
@@ -447,14 +453,14 @@ Section StateRepProperties.
              destruct Hcoal1 as [Hcoal1 Hcoal2].
 
              apply sep_imp'.
-             + destruct a.
+             + destruct a; simpl. 
                destruct (field_offset gcenv i (co_members co)) eqn:Hfo; auto.
                rewrite match_value_empty.
                rewrite sizeof_translate_chunk.
                *{ apply range_contains'.
                   specialize (Htype i t).
                   rewrite <-Hmem in Htype.
-                  apply field_offset_aligned with (ty:=t) in Hfo.
+                  apply field_offset_aligned with (ty:=cltype t) in Hfo.
                   - simpl in Hcoal1.
                     apply Z.divide_add_r.
                     + apply Zdivide_trans with (2:=Halign).
@@ -545,13 +551,13 @@ Section StateRepProperties.
   Qed.
 
   Lemma staterep_deref_mem:
-    forall cls prog' m me ve b ofs x ty d v P,
-      access_mode ty = By_value (chunk_of_type ty) ->
+    forall cls prog' m me b ofs x ty d v P,
+      access_mode (cltype ty) = By_value (chunk_of_type ty) ->
       m |= staterep gcenv (cls::prog') cls.(c_name) me b ofs ** P ->
       In (x, ty) cls.(c_mems) ->
-      find_field (me, ve) x v ->
+      mfind_mem x me = Some v ->
       field_offset gcenv x (make_members cls) = Errors.OK d ->
-      Clight.deref_loc ty m b (Int.repr (ofs + d)) v.
+      Clight.deref_loc (cltype ty) m b (Int.repr (ofs + d)) v.
   Proof.
     intros ** Hty Hm Hin Hv Hoff.
     apply sep_proj1 in Hm.
@@ -566,23 +572,23 @@ Section StateRepProperties.
     apply loadv_rule in Hm.
     destruct Hm as [v' [Hloadv Hmatch]].
     unfold match_value in Hmatch.
-    unfold find_field, mfind_mem in Hv; simpl in Hv.
-    rewrite Hv in Hmatch. clear Hv.
-    rewrite Hmatch in Hloadv. clear Hmatch.
+    unfold mfind_mem in Hv; simpl in Hv.
+    rewrite Hv in Hmatch; clear Hv.
+    rewrite Hmatch in Hloadv; clear Hmatch.
     apply Clight.deref_loc_value with (2:=Hloadv); auto.
   Qed.
 
   Lemma staterep_assign_mem:
     forall P cls prog' m m' me b ofs x ty d v,
       (P me -*> P (madd_mem x v me)) ->
-      access_mode ty = By_value (chunk_of_type ty) ->
+      access_mode (cltype ty) = By_value (chunk_of_type ty) ->
       NoDup cls.(c_objs) ->
       NoDupMembers cls.(c_mems) ->
       m |= staterep gcenv (cls::prog') cls.(c_name) me b ofs ** P me ->
       In (x, ty) cls.(c_mems) ->
       field_offset gcenv x (make_members cls) = Errors.OK d ->
       v = Values.Val.load_result (chunk_of_type ty) v ->
-      Clight.assign_loc gcenv ty m b (Int.repr (ofs + d)) v m' ->
+      Clight.assign_loc gcenv (cltype ty) m b (Int.repr (ofs + d)) v m' ->
       m' |= staterep gcenv (cls::prog') cls.(c_name) (madd_mem x v me) b ofs
                ** P (madd_mem x v me).
   Proof.
@@ -600,7 +606,7 @@ Section StateRepProperties.
     rewrite Hoff in *.
     rewrite sep_swap2.
     rewrite sepall_switchp
-    with (f':=fun xty : ident * typ =>
+    with (f':=fun xty : ident * type =>
                 let (x0, ty0) := xty in
                 match field_offset gcenv x0 (make_members cls) with
                 | Errors.OK d0 =>
@@ -619,7 +625,7 @@ Section StateRepProperties.
     - apply NoDupMembers_remove_1 in Hmem.
       apply NoDupMembers_NoDup with (1:=Hmem).
     - intros x' Hin'; destruct x' as [x' ty'].
-      unfold update_field, madd_mem; simpl.
+      unfold madd_mem; simpl.
       rewrite match_value_add; [reflexivity|].
       apply NoDupMembers_app_cons in Hmem.
       destruct Hmem as [Hmem].
@@ -702,8 +708,8 @@ Section BlockRep.
   Hypothesis ge_consistent : composite_env_consistent ge.
 
   (* TODO: name predicate "blockrep" and write sepall blockrep xs *)
-  Definition blockrep (ve: venv) (flds: members) (b: block) : massert :=
-    sepall (fun xty : ident * type =>
+  Definition blockrep (ve: stack) (flds: members) (b: block) : massert :=
+    sepall (fun xty : ident * Ctypes.type =>
               let (x, ty) := xty in
               match field_offset ge x flds, access_mode ty with
               | Errors.OK d, By_value chunk =>
@@ -867,7 +873,7 @@ Section BlockRep.
 
   Lemma blockrep_any_empty:
     forall flds ve b,
-      blockrep ve flds b -*> blockrep v_empty flds b.
+      blockrep ve flds b -*> blockrep sempty flds b.
   Proof.
     intros flds ve b.
     apply sepall_weakenp.
@@ -903,12 +909,12 @@ Section BlockRep.
       eapply In_InMembers; eauto.
   Qed.
 
-    Lemma blockrep_findvars:
-    forall S xs vs b,
-      find_vars S xs vs ->
-      blockrep (snd S) xs b -*> blockrep (adds xs vs v_empty) xs b.
+  Lemma blockrep_findvars:
+    forall ve xs vs b,
+      Forall2 (fun xty v => PM.find (fst xty) ve = Some v) xs vs ->
+      blockrep ve xs b -*> blockrep (adds xs vs sempty) xs b.
     Proof.
-      destruct S as (?, ve); unfold find_vars, find_var, adds; simpl.
+      unfold  adds; simpl.
       intros ** Findvars.
       unfold blockrep.
       apply sepall_weakenp.
@@ -921,9 +927,9 @@ Section BlockRep.
       revert vs Findvars.
       induction xs as [|(x', t')], vs; simpl; intro Findvars;
       try (rewrite PM.gempty; auto).
-      inversion Findvars as [|y ? ys ? Find Findvars' Heq]; subst; clear Findvars.
+      inversion Findvars as [|y ? ys ? Find Findvars']; subst; clear Findvars.
       destruct (split xs) as (g, d).
-      simpl in *; inv Heq.
+      simpl in *.
       destruct (ident_eqb x x') eqn: E.
       - apply ident_eqb_eq in E; subst x'.
         rewrite Find in Findx.
