ObcToClight/Translation.v
@@ -2,27 +2,28 @@ Require cfrontend.Clight.
 Require Import lib.Integers.
 
 Require Import Rustre.Common.
-Require Import Rustre.Nelist.
+Require Import Rustre.Obc.Syntax.
+Require Import Rustre.ObcToClight.Interface.
+Require Import Rustre.Ident.
+Require Import Operators.
 
-Require Import Syn.
+Module Export OpAux := OperatorsAux Op.
+Module Export Syn := SyntaxFun Ids Op OpAux.
 
 Require Import String.
 Require Import List.
 Import List.ListNotations.
 Open Scope list_scope.
 
-Axiom pos_to_str: ident -> string.
-
 Definition main_id: ident := pos_of_str "main".
 Axiom prefix: ident -> ident -> ident.
 Axiom fun_id: ident.
-(* Axiom out_id: ident. *)
-Axiom fun_not_out: fun_id <> out_id.
+Axiom fun_not_out: fun_id <> out.
 
 Definition prefix_fun (c f: ident): ident :=
   prefix fun_id (prefix c f).
 Definition prefix_out (o f: ident): ident :=
-  prefix out_id (prefix o f).
+  prefix out (prefix o f).
 
 Axiom prefix_injective:
   forall pref id pref' id',
@@ -52,60 +53,77 @@ Definition step_id (id: ident): ident :=
 (*   pos_of_str ("reset_" ++ (pos_to_str id)). *)
 
 (* TRANSLATION *)
-Definition type_of_inst (o: ident): typ :=
+Definition type_of_inst (o: ident): Ctypes.type :=
   Ctypes.Tstruct o Ctypes.noattr.
-Definition pointer_of (ty: typ): typ :=
+Definition pointer_of (ty: Ctypes.type): Ctypes.type :=
   Ctypes.Tpointer ty Ctypes.noattr.
-Definition type_of_inst_p (o: ident): typ :=
+Definition type_of_inst_p (o: ident): Ctypes.type :=
   pointer_of (type_of_inst o).
 
-Definition deref_field (id cls x: ident) (xty: typ): Clight.expr :=
+Definition deref_field (id cls x: ident) (xty: Ctypes.type): Clight.expr :=
   let ty_deref := type_of_inst cls in
   let ty_ptr := pointer_of ty_deref in
   Clight.Efield (Clight.Ederef (Clight.Etempvar id ty_ptr) ty_deref) x xty.
 
-Definition translate_const (c: const): typ -> Clight.expr :=
-  match c with
-  | Cint i => Clight.Econst_int i
+Definition translate_const (c: const): Clight.expr :=
+  (match c with
+  | Cint i _ _ => Clight.Econst_int i
+  | Clong l _ => Clight.Econst_long l
   | Cfloat f => Clight.Econst_float f
   | Csingle s => Clight.Econst_single s
-  | Clong l => Clight.Econst_long l
+  end) (cltype (type_const c)).
+
+Definition translate_unop (op: unop) (e: Clight.expr) (ty: Ctypes.type): Clight.expr :=
+  match op with
+  | UnaryOp cop => Clight.Eunop cop e ty
+  | CastOp ty => Clight.Ecast e (cltype ty)
   end.
+
+Definition translate_binop (op: binop): Clight.expr -> Clight.expr -> Ctypes.type -> Clight.expr :=
+  Clight.Ebinop op.
 
 (** Straightforward expression translation *)
-Definition translate_exp (c: class) (m: method) (e: exp): Clight.expr :=
+Fixpoint translate_exp (c: class) (m: method) (e: exp): Clight.expr :=
   match e with
   | Var x ty =>
+    let ty := cltype ty in
     if existsb (fun out => ident_eqb (fst out) x) m.(m_out) then
-      deref_field out_id (prefix_fun c.(c_name) m.(m_name)) x ty
+      deref_field out (prefix_fun c.(c_name) m.(m_name)) x ty
     else
       Clight.Etempvar x ty  
-  | State x ty => deref_field self_id c.(c_name) x ty
-  | Const c ty => translate_const c ty
+  | State x ty =>
+    deref_field self c.(c_name) x (cltype ty)
+  | Const c =>
+    translate_const c
+  | Unop op e ty =>
+    translate_unop op (translate_exp c m e) (cltype ty)
+  | Binop op e1 e2 ty =>
+    translate_binop op (translate_exp c m e1) (translate_exp c m e2) (cltype ty)
   end.
 
-Fixpoint list_type_to_typelist (tys: list typ): Ctypes.typelist :=
+Fixpoint list_type_to_typelist (tys: list Ctypes.type): Ctypes.typelist :=
   match tys with
   | [] => Ctypes.Tnil
   | ty :: tys => Ctypes.Tcons ty (list_type_to_typelist tys)
   end.
 
 Definition funcall (f: ident) (args: list Clight.expr) : Clight.statement :=
-  let tys := List.map Clight.typeof args in
+  let tys := map Clight.typeof args in
   let sig := Ctypes.Tfunction (list_type_to_typelist tys) Ctypes.Tvoid AST.cc_default in
   Clight.Scall None (Clight.Evar f sig) args.
 
-Definition assign (x: ident) (ty: typ) (clsid: ident) (m: method): Clight.expr -> Clight.statement :=
+Definition assign (x: ident) (ty: Ctypes.type) (clsid: ident) (m: method): Clight.expr -> Clight.statement :=
   if existsb (fun out => ident_eqb (fst out) x) m.(m_out) then
-    Clight.Sassign (deref_field out_id (prefix_fun clsid m.(m_name)) x ty)
+    Clight.Sassign (deref_field out (prefix_fun clsid m.(m_name)) x ty)
   else
     Clight.Sset x.
 
 Definition ptr_obj (owner: ident) (cls obj: ident): Clight.expr :=
-  Clight.Eaddrof (deref_field self_id owner obj (type_of_inst cls)) (type_of_inst_p cls).  
+  Clight.Eaddrof (deref_field self owner obj (type_of_inst cls)) (type_of_inst_p cls).  
 
 Definition funcall_assign
-           (ys: list (ident * typ)) (owner: ident) (caller: method) (obj: ident) (tyout: typ) (callee: method)
+           (ys: list (ident * Ctypes.type)) (owner: ident) (caller: method)
+           (obj: ident) (tyout: Ctypes.type) (callee: method)
            : Clight.statement :=
   fold_right
     (fun y s =>
@@ -115,8 +133,8 @@ Definition funcall_assign
     ) Clight.Sskip (combine ys callee.(m_out)).
 
 Definition binded_funcall
-           (prog: program) (ys: list (ident * typ)) (owner: ident) (caller: method)
-           (cls obj f: ident) (args: list Clight.expr)
+           (prog: program) (ys: list (ident * Ctypes.type)) (owner: ident)
+           (caller: method) (cls obj f: ident) (args: list Clight.expr)
   : Clight.statement :=
   match find_class cls prog with
   | Some (c, _) =>
@@ -133,6 +151,10 @@ Definition binded_funcall
   | None => Clight.Sskip
   end.
 
+Definition translate_param (yt: ident * type): ident * Ctypes.type :=
+  let (y, t) := yt in
+  (y, cltype t).
+
 (** 
 Statement conversion keeps track of the produced temporaries (function calls).
 [c] represents the current class.
@@ -141,14 +163,15 @@ Fixpoint translate_stmt (prog: program) (c: class) (m: method) (s: stmt)
   : Clight.statement :=
   match s with
   | Assign x e =>
-    assign x (typeof e) c.(c_name) m (translate_exp c m e)
+    assign x (cltype (typeof e)) c.(c_name) m (translate_exp c m e)
   | AssignSt x e =>
-    Clight.Sassign (deref_field self_id c.(c_name) x (typeof e)) (translate_exp c m e)
+    Clight.Sassign (deref_field self c.(c_name) x (cltype (typeof e))) (translate_exp c m e)
   | Ifte e s1 s2 =>
     Clight.Sifthenelse (translate_exp c m e) (translate_stmt prog c m s1) (translate_stmt prog c m s2) 
   | Comp s1 s2 =>
     Clight.Ssequence (translate_stmt prog c m s1) (translate_stmt prog c m s2)
   | Call ys cls o f es =>
+    let ys := map translate_param ys in
     binded_funcall prog ys c.(c_name) m cls o f (map (translate_exp c m) es)  
   | Skip => Clight.Sskip
   end.
@@ -164,19 +187,21 @@ Definition return_zero (s: Clight.statement): Clight.statement :=
   Clight.Ssequence s (Clight.Sreturn (Some cl_zero)).
 
 Definition fundef
-           (ins: list (ident * typ)) (vars temps: list (ident * typ)) (ty: typ) (body: Clight.statement)
+           (ins: list (ident * Ctypes.type)) (vars temps: list (ident * Ctypes.type))
+           (ty: Ctypes.type) (body: Clight.statement)
   : AST.globdef Clight.fundef Ctypes.type :=
   let f := Clight.mkfunction ty AST.cc_default ins vars temps body in
-  @AST.Gfun Clight.fundef typ (Ctypes.Internal f).
+  @AST.Gfun Clight.fundef Ctypes.type (Ctypes.Internal f).
 
 Definition make_fundef
-           (self: ident * typ) (ins: list (ident * typ)) (out: ident * typ)
-           (vars temps: list (ident * typ)) (body: Clight.statement)
+           (self: ident * Ctypes.type) (ins: list (ident * Ctypes.type))
+           (out: ident * Ctypes.type) (vars temps: list (ident * Ctypes.type))
+           (body: Clight.statement)
   : AST.globdef Clight.fundef Ctypes.type :=
   let body := return_none body in
   fundef (self :: out :: ins) vars temps Ctypes.Tvoid body.
 
-Definition make_out_vars (out_vars: list (ident * ident * ident)): list (ident * typ) :=
+Definition make_out_vars (out_vars: list (ident * ident * ident)): list (ident * Ctypes.type) :=
   map (fun ofc =>
          let '(o, f, cid) := ofc in
          (prefix_out o f, type_of_inst (prefix_fun cid f))
@@ -201,27 +226,33 @@ Definition translate_method (prog: program) (c: class) (m: method)
   : ident * AST.globdef Clight.fundef Ctypes.type :=
   let body := translate_stmt prog c m m.(m_body) in
   let out_vars := instance_methods m in
-  let self := (self_id, type_of_inst_p c.(c_name)) in
-  let out := (out_id, type_of_inst_p (prefix_fun c.(c_name) m.(m_name))) in
+  let self := (self, type_of_inst_p c.(c_name)) in
+  let ins := map translate_param m.(m_in) in
+  let out := (out, type_of_inst_p (prefix_fun c.(c_name) m.(m_name))) in
+  let vars := map translate_param m.(m_vars) in
   (prefix_fun c.(c_name) m.(m_name),
-   make_fundef self m.(m_in) out (make_out_vars out_vars) m.(m_vars) body).
+   make_fundef self ins out (make_out_vars out_vars) vars body).
 
 Definition make_methods (prog: program) (c: class)
   : list (ident * AST.globdef Clight.fundef Ctypes.type) :=
   map (translate_method prog c) c.(c_methods).
 
-Definition translate_obj (obj: ident * ident): (ident * typ) :=
+Definition translate_obj (obj: ident * ident): (ident * Ctypes.type) :=
   let (o, c) := obj in
   (o, type_of_inst c).
 
 Definition make_members (c: class): Ctypes.members :=
-  c.(c_mems) ++ map translate_obj c.(c_objs).
+  map translate_param c.(c_mems) ++ map translate_obj c.(c_objs).
 
 Definition make_struct (c: class): Ctypes.composite_definition :=
   Ctypes.Composite c.(c_name) Ctypes.Struct (make_members c) Ctypes.noattr.
 
 Definition translate_out (c: class) (m: method): Ctypes.composite_definition :=
-  Ctypes.Composite (prefix_fun c.(c_name) m.(m_name)) Ctypes.Struct m.(m_out) Ctypes.noattr.
+  Ctypes.Composite
+    (prefix_fun c.(c_name) m.(m_name))
+    Ctypes.Struct
+    (map translate_param m.(m_out))
+    Ctypes.noattr.
 
 Definition make_out (c: class): list Ctypes.composite_definition :=
   map (translate_out c) c.(c_methods).
@@ -235,11 +266,11 @@ Definition translate_class (prog: program) (c: class)
 
 Definition glob_id (id: ident): ident :=
   pos_of_str ("_" ++ (pos_to_str id)).
-Definition glob_bind (bind: ident * typ): ident * typ :=
+Definition glob_bind (bind: ident * type): ident * Ctypes.type :=
   let (x, ty) := bind in
-  (glob_id x, ty).
+  (glob_id x, cltype ty).
 
-Definition make_in_arg (arg: ident * typ): Clight.expr :=
+Definition make_in_arg (arg: ident * Ctypes.type): Clight.expr :=
   let (x, ty) := arg in
   Clight.Evar x ty.
 (* Definition make_out_arg (arg: ident * typ): Clight.expr := *)
@@ -247,11 +278,11 @@ Definition make_in_arg (arg: ident * typ): Clight.expr :=
 (*   Clight.Eaddrof (Clight.Evar x ty) (pointer_of ty). *)
 
 Definition make_main
-           (prog: program) (node: ident) (ins: list (ident * typ))
-           (outs: list (ident * typ)) (m: method)
+           (prog: program) (node: ident) (ins: list (ident * Ctypes.type))
+           (outs: list (ident * Ctypes.type)) (m: method)
   : AST.globdef Clight.fundef Ctypes.type :=
   let out_struct := step_id node in
-  let args_in := List.map make_in_arg ins in
+  let args_in := map make_in_arg ins in
   let tyout := type_of_inst (step_id node) in
   let out := Clight.Eaddrof (Clight.Evar out_struct tyout) (pointer_of tyout) in 
   let args := (Clight.Eaddrof (Clight.Evar (glob_id node) (type_of_inst node)) (type_of_inst_p node))
@@ -264,12 +295,13 @@ Definition make_main
                       let assign_out := Clight.Sassign (Clight.Evar y ty)
                                                        (Clight.Efield (Clight.Evar out_struct tyout) y' ty) in
                       Clight.Ssequence assign_out s
-    ) Clight.Sskip (combine outs m.(m_out))) in
+                   ) Clight.Sskip (combine outs m.(m_out))) in
   let loop := Clight.Sloop ((* Clight.Ssequence wait *) step) Clight.Sskip in
   let body := return_zero ((* Clight.Ssequence (reset_call None node f) *) loop) in
   fundef [] [(out_struct, type_of_inst (step_id node))] [] Ctypes.type_int32s body.
 
-Definition vardef (init volatile: bool) (x: ident * typ): ident * AST.globdef Clight.fundef Ctypes.type :=
+Definition vardef (init volatile: bool) (x: ident * Ctypes.type)
+  : ident * AST.globdef Clight.fundef Ctypes.type :=
   let (x, ty) := x in
   let ty' := Ctypes.merge_attributes ty (Ctypes.mk_attr volatile None) in
   (x, @AST.Gvar Clight.fundef _
@@ -308,7 +340,7 @@ Definition translate (prog: program) (main_node: ident): Errors.res Clight.progr
       let ins := map glob_bind m.(m_in) in
       let outs := map glob_bind m.(m_out) in
       let main := make_main prog main_node ins outs m in
-      let cs := List.map (translate_class prog) prog in
+      let cs := map (translate_class prog) prog in
       let f_gvar := vardef true false (f, type_of_inst main_node) in
       let o_gvars := map (vardef true true) outs in
       let i_gvars := map (vardef true true) ins in
