Ident.v
@@ -1,0 +1,25 @@
+Require Import Rustre.Common.
+Require Import String.
+Require Import List.
+Import List.ListNotations.
+
+Axiom pos_to_str: ident -> string.
+Axiom pos_of_str: string -> ident.
+
+Module Export Ids <: IDS.
+  Definition self := pos_of_str "self".
+  Definition out := pos_of_str "out".             
+
+  Definition step := pos_of_str "step".
+  Definition reset := pos_of_str "reset".
+
+  Definition reserved : list ident := [ self; out ].
+
+  Definition methods  : list ident := [ step; reset ].
+
+  Lemma reserved_nodup: NoDup reserved. Admitted.
+  Lemma methods_nodup: NoDup methods. Admitted.
+
+  Definition NotReserved {typ: Type} (xty: ident * typ) : Prop :=
+    ~In (fst xty) reserved.
+End Ids.
